Completeness theorem for Core Simplicity.

Coq/Simplicity/Core.v
@@ -28,3 +28,71 @@ match x in Term A B return tySem A -> tySem B with
 | take t => fun ab => eval t (fst ab)
 | drop t => fun ab => eval t (snd ab)
 end.
+
+Section Completeness.
+
+Fixpoint scribe {A B : Ty} : B -> Term A B :=
+match B with
+| Unit => fun _ => unit
+| Sum BL BR => fun b =>
+  match b with
+  | inl l => injl (scribe l)
+  | inr r => injr (scribe r)
+  end
+| Prod B1 B2 => fun b => pair (scribe (fst b)) (scribe (snd b))
+end.
+
+Lemma scribe_correct (A B : Ty) (a : A) (b : B) : eval (scribe b) a = b.
+Proof.
+induction B.
+- destruct b; reflexivity.
+- destruct b as [b|b];cbn;f_equal;auto.
+- destruct b as [b0 b1];cbn;f_equal;auto.
+Qed.
+
+Fixpoint reifyProd {A B C : Ty} : (A -> Term B C) -> Term (Prod A B) C :=
+match A with
+| Unit => fun f => drop (f tt)
+| Sum AL AR => fun f => case (reifyProd (fun al => f (inl al)))
+                             (reifyProd (fun ar => f (inr ar)))
+| Prod A1 A2 => fun f => comp (pair (take (take iden))
+                                    (pair (take (drop iden)) (drop iden)))
+                         (reifyProd (fun a1 => reifyProd (fun a2 => f (a1, a2))))
+end.
+
+Lemma reifyProd_correct : forall (A B C : Ty) (f : A -> Term B C) (a : A) (b : B),
+  eval (reifyProd f) (a, b) = eval (f a) b.
+Proof.
+intros A.
+induction A; intros B C f a b.
+- destruct a; reflexivity.
+- destruct a as [a|a];cbn;[rewrite IHA1|rewrite IHA2];reflexivity.
+- destruct a as [a1 a2];cbn;rewrite IHA1, IHA2;reflexivity.
+Qed.
+
+Fixpoint reify {A B : Ty} : (A -> B) -> Term A B :=
+match A with
+| Unit => fun f => scribe (f tt)
+| Sum AL AR => fun f => comp (pair iden unit)
+                             (case (take (reify (fun al => f (inl al))))
+                                   (take (reify (fun ar => f (inr ar)))))
+| Prod A1 A2 => fun f => reifyProd (fun a1 => reify (fun a2 => f (a1, a2)))
+end.
+
+Lemma reify_correct (A B : Ty) (f : A -> B) (a : A) : eval (reify f) a = f a.
+Proof.
+induction A.
+- destruct a; cbn; apply scribe_correct.
+- destruct a as [a|a];cbn;[apply IHA1|apply IHA2].
+- destruct a as [a0 a1]; cbn; rewrite reifyProd_correct; apply IHA2.
+Qed.
+
+Theorem Simplicity_Completeness : forall (A B : Ty) (f : A -> B),
+  { t : Term A B | forall a, eval t a = f a }.
+Proof.
+intros A B f.
+exists (reify f).
+apply reify_correct.
+Defined.
+
+End Completeness.
